\documentclass[12pt]{article}

\begin{document}

\begin{eqnarray*}
T_{pq} = T_{ij} & = & \frac{q_j}{r^3} (\vec{p_i} \times \vec{r}) \\
T_{qp} = T_{ji} & = & - \frac{q_i}{r^3} (\vec{p_j} \times \vec{r}) \\
T_{pp} = T_{ij} & = & -\frac{1}{r^3} (\vec{p_i} \times \vec{p_j}) + 
                      \frac{3}{r^5} (\vec{p_j} \bullet \vec{r})
		      (\vec{p_i} \times \vec{r}) \\
T_{pp} = T_{ji} & = & -\frac{1}{r^3} (\vec{p_j} \times \vec{p_i}) + 
                      \frac{3}{r^5} (\vec{p_i} \bullet \vec{r}) 
		      (\vec{p_j} \times \vec{r}) \\
\end{eqnarray*}                                                  

\end{document}
